Veritas.StateSeqMachine.fsti
@@ -1,0 +1,34 @@
+module Veritas.StateSeqMachine
+
+open FStar.Seq
+open Veritas.Record
+open Veritas.State
+open Veritas.SeqMachine
+
+type ssm_state = 
+  | StateInit: ssm_state
+  | StateVal: v:data_value -> ssm_state
+  | StateFail: ssm_state
+
+let apply_state_op (o: state_op) (s: ssm_state) = 
+  match s with
+  | StateFail -> StateFail
+  | StateInit -> (match o with 
+                  | Get _ v ->  if v = Null then StateVal v
+                                else StateFail
+                  | Put _ v -> StateVal v
+                 )
+  | StateVal v -> (match o with
+                  | Get _ v' -> if v = v' then s
+                                else StateFail
+                  | Put _ v' -> StateVal v'
+                  )
+
+let ssm_k = SeqMachine StateInit StateFail apply_state_op
+
+(* state seq machine *)
+let ssm = PSM ssm_k key_of
+
+(* validity under state seq machine is equivalent to rw_consistency *)
+val lemma_state_sm_equiv_rw_consistent (s: seq state_op):
+  Lemma (valid_all ssm s <==> rw_consistent s)
